WIP add sort of the addresses when hashing the memory

theories/cap_lang.v
@@ -2,6 +2,7 @@ From iris.prelude Require Import prelude.
 From iris.program_logic Require Import language ectx_language ectxi_language.
 From stdpp Require Import gmap fin_maps list.
 From cap_machine Require Export addr_reg machine_base machine_parameters.
+From Coq Require Import Sorting Orders.
 Set Warnings "-redundant-canonical-projection".
 
 Ltac inv H := inversion H; clear H; subst.
@@ -401,6 +402,23 @@ Proof.
   ; [eapply sweep_registers_addr_spec | eapply sweep_memory_addr_spec].
 Qed.
 
+
+Module MemOrder <: TotalLeBool.
+  Definition t : Type := (Addr * Word).
+  Definition leb (aw1 aw2 : t) :=
+    ((aw1).1 <=? (aw2).1)%a.
+  Infix "<=?" := leb (at level 70, no associativity).
+  Theorem leb_total : forall a1 a2 : t, ( (a1 <=? a2) = true \/ (a2 <=? a1) = true).
+  Proof.
+    destruct a1 as [a1 w1], a2 as [a2 w2].
+    rewrite /leb /finz.leb ; cbn.
+    pose proof (Zle_bool_total a1 a2).
+    destruct H ; [by left|by right].
+  Qed.
+End MemOrder.
+Module Import MemSort := Sort MemOrder.
+
+
 Section opsem.
   Context `{MachineParameters}.
 
@@ -454,11 +472,12 @@ Section opsem.
   Definition otype_has_seal (ot : OType) (tid : TIndex) : Prop :=
     tid_of_otype ot = Some tid.
 
+
   Definition hash_memory_region (m : Mem) (b e : Addr) :=
     let instructions : list Word :=
       snd <$>
-        ((map_to_list
-            (filter (fun '(a, _) => a ∈ (finz.seq_between b e)) m)))
+        (sort ((map_to_list
+                  (filter (fun '(a, _) => a ∈ (finz.seq_between b e)) m))))
     in
     hash instructions.
 
